ems/SimModSem.v
@@ -1018,7 +1018,7 @@ Import ModSem.
 
 Definition wf_lift {world} wf  :=
   fun (w:world) => 
-  (fun '(src, tgt) =>
+  (fun '(src, tgt) => 
     match (Any.split src), (Any.split tgt) with
     | Some (l1, r1), Some (l2, r2) => ( wf w (l1, l2) /\ r1 = r2)
     | _, _ => False
@@ -1237,28 +1237,104 @@ Proof.
       gfinal. left. eapply CIH; et.
 Qed.
 
+Lemma sim_itree_init
+  {world} wf (le: relation world) ps pt w sts stt stctx (its itt: itree eventE Any.t)
+  (SIM: sim_itree wf le [] [] ps pt w (sts, resum_itr its) (stt, resum_itr itt))
+:
+  paco8 (_sim_itree (wf_lift wf) le [] []) bot8 Any.t Any.t
+  (@lift_rel world (wf_lift wf) le Any.t Any.t w eq) ps pt w
+  (Any.pair sts stctx, resum_itr its) (Any.pair stt stctx, resum_itr itt).
+Proof. 
+  remember (resum_itr its) as itrs.
+  remember (resum_itr itt) as itrt.
+  revert_until wf. cofix CIH. i.
+  remember (sts, itrs) as stis.
+  remember (stt, itrt) as stit.
+  remember w eqn:Weq.
+  unfold sim_itree in SIM.
+  rewrite Weq in SIM at 2.
+  move SIM before le. revert_until SIM.
+  pattern ps, pt, w, stis, stit.
+  match goal with
+  | |- ?P ps pt w stis stit => set P
+  end.
+  Local Transparent resum_itr.
+  eapply (@sim_itree_ind world wf le [] [] Any.t Any.t (lift_rel wf le w0 (@eq Any.t)) P); subst P; ss; i; des; clarify; try (rewrite <- H0; rewrite <- H1).
+  - pstep. econs. unfold lift_rel in *. des. subst. esplits; eauto.
+    r. rewrite !Any.pair_split. esplits; eauto.
+  - rewrite bind_trigger in H0. ides itt.
+    + rewrite resum_itr_ret in H0. inv H0.
+    + rewrite resum_itr_tau in H0. inv H0.
+    + destruct e; unfold resum_itr in H0; erewrite ! (bisimulation_is_eq _ _ (interp_vis _ _ _)) in H0;
+      rewrite bind_trigger in H0; inv H0.
+  - rewrite bind_trigger in H0. ides itt.
+    + rewrite resum_itr_ret in H0. inv H0.
+    + rewrite resum_itr_tau in H0. inv H0.
+    + destruct e; unfold resum_itr in H0; erewrite ! (bisimulation_is_eq _ _ (interp_vis _ _ _)) in H0;
+      rewrite bind_trigger in H0; inv H0.
+      pstep. econs. i. econs. unfold upaco8. left. eapply CIH.
+      2: { eapply inj_pair2 in H5. eapply equal_f in H5.
+        rewrite H5. unfold resum_itr.
+        Check 
+      }
+      (**** TODO: Show that ktr is also 'resum_itr (itree eventE _)' ****)
+      3: { unfold sim_itree. eapply sim_itree_bot_flag_up. eapply K. } 
+      all: admit.   
+  - ides its.
+    + rewrite resum_itr_ret in H0. inv H0.
+    + rewrite resum_itr_tau in H0. inv H0.
+      ginit. rewrite resum_itr_tau. eapply sim_itreeC_spec. econs.
+      gfinal. right. eapply IH; eauto.
+    + destruct e; unfold resum_itr in H0; erewrite ! (bisimulation_is_eq _ _ (interp_vis _ _ _)) in H0;
+      rewrite bind_trigger in H0; inv H0.
+  - ides itt.
+    + rewrite resum_itr_ret in H0. inv H0.
+    + rewrite resum_itr_tau in H0. inv H0.
+      ginit. rewrite resum_itr_tau. eapply sim_itreeC_spec. econs.
+      gfinal. right. eapply IH; eauto.
+    + destruct e; unfold resum_itr in H0; erewrite ! (bisimulation_is_eq _ _ (interp_vis _ _ _)) in H0;
+      rewrite bind_trigger in H0; inv H0.
+  - admit.
+  - admit.
+  - admit.
+  - admit.
+  - rewrite bind_trigger in H0. ides its.
+    + rewrite resum_itr_ret in H0. inv H0.
+    + rewrite resum_itr_tau in H0. inv H0.
+    + destruct e; unfold resum_itr in H0; erewrite ! (bisimulation_is_eq _ _ (interp_vis _ _ _)) in H0;
+      rewrite bind_trigger in H0; inv H0.
+  - rewrite bind_trigger in H0. ides itt.
+    + rewrite resum_itr_ret in H0. inv H0.
+    + rewrite resum_itr_tau in H0. inv H0.
+    + destruct e; unfold resum_itr in H0; erewrite ! (bisimulation_is_eq _ _ (interp_vis _ _ _)) in H0;
+      rewrite bind_trigger in H0; inv H0.
+  - pstep. econs. left. eapply CIH; eauto. 
+Admitted.
+
 Theorem sim_ctx
       ctx ms1 ms2
       (SIM: ModSemPair.sim ms1 ms2)
     :
       ModSemPair.sim (add ms1 ctx) (add ms2 ctx)
 .
-Proof. Admitted.
-  (* inv SIM. inv sim_initial.
+Proof.
+ (* Admitted. *)
+  inv SIM. inv sim_initial.
   econs; et; cycle 1.
   { exists x.
-    admit.
+    (* admit. *)
     (****** require different 'wf' in head & continuation? ******)
-   (* instantiate (1:= wf_lift wf0). s. *)
-    (* s. rewrite ! resum_itr_bind. ginit. guclo lbindC_spec. econs.
-    { gfinal. right. et. }
-    i. rewrite ! resum_itr_bind. guclo lbindC_spec. econs.
-    { admit. }
+   instantiate (1:= wf_lift wf0). s.
+   (* instantiate (1:= fun ) *)
+    s. rewrite ! resum_itr_bind. ginit. guclo lbindC_spec. econs.
+    { gfinal. right. eapply sim_itree_init. eauto. }
+    i. rr in SIM. des. subst. rr in SIM0.
+    rewrite !Any.pair_split in SIM0. des.
     i.
     gfinal. right. exploit self_sim_itree. eapply self_sim_itree.
     Search resum_itr.    
     rewrite ! Any.pair_split.
-    splits; et. *)
+    splits; et.
   }
   s. unfold add_fnsems, trans_l, trans_r.
   apply Forall2_app; eapply Forall2_apply_Forall2; et; cycle 1.
@@ -1339,6 +1415,6 @@ Proof. Admitted.
     specialize H1 with (x:=y) (y:=y) (w:=w) (mrs_src := t0) (mrs_tgt := t2).
     specialize (H1 eq_refl SIMMRS).
     eapply sim_ctx_aux; et.
-Qed. *)
+Qed.
 
 End SIMCTX.
